RBT_Ex.thy
@@ -2,6 +2,8 @@ theory RBT_Ex
 imports Auto2 Lists_Ex
 begin
 
+section {* Definition of RBT, and basic setup *}
+
 datatype color = R | B
 datatype 'a pre_rbt =
     Leaf
@@ -10,40 +12,28 @@ where
   "cl Leaf = B"
 
 setup {* fold add_rew_const [@{term "R"}, @{term "B"}, @{term "Leaf"}] *}
-setup {* fold add_rewrite_rule [@{thm pre_rbt.sel(2)}, @{thm pre_rbt.sel(3)}] *}
-setup {* add_simp_rule_cond @{thm pre_rbt.sel(1)} [with_cond "?x21.0 \<noteq> lsub ?t"] *}
-setup {* add_simp_rule_cond @{thm pre_rbt.sel(5)} [with_cond "?x24.0 \<noteq> rsub ?t"] *}
+setup {* add_resolve_prfstep @{thm color.distinct(1)} *}
+setup {* add_resolve_prfstep @{thm pre_rbt.distinct(2)} *}
+setup {* fold add_rewrite_rule @{thms pre_rbt.sel} *}
 
-(* Case checking. *)
+text {* Case checking: after checking the Leaf case, can assume t is in the
+  form Node l c n r. *}
+
 setup {* add_gen_prfstep ("rbt_case_intro",
      [WithTerm @{term_pat "?t::?'a pre_rbt"},
       Filter (unique_free_filter "t"),
       CreateCase ([@{term_pat "(?t::?'a pre_rbt) = Leaf"}], [])]) *}
+setup {* add_forward_prfstep @{thm pre_rbt.collapse} *}
 
-setup {* add_forward_prfstep @{thm pre_rbt.collapse} *}  (* Case checking after Leaf case. *)
-setup {* add_resolve_prfstep @{thm color.distinct(1)} *}
-setup {* add_resolve_prfstep @{thm pre_rbt.distinct(2)} *}
+text {* Induction: after checking the Leaf case, can assume P (lsub t) and
+  P (rsub t) holds when proving P t. *}
 
-abbreviation LL :: "'a pre_rbt \<Rightarrow> 'a pre_rbt" where "LL t \<equiv> lsub (lsub t)"
-abbreviation LR :: "'a pre_rbt \<Rightarrow> 'a pre_rbt" where "LR t \<equiv> rsub (lsub t)"
-abbreviation RL :: "'a pre_rbt \<Rightarrow> 'a pre_rbt" where "RL t \<equiv> lsub (rsub t)"
-abbreviation RR :: "'a pre_rbt \<Rightarrow> 'a pre_rbt" where "RR t \<equiv> rsub (rsub t)"
-abbreviation LLL :: "'a pre_rbt \<Rightarrow> 'a pre_rbt" where "LLL t \<equiv> LL (lsub t)"
-abbreviation LLR :: "'a pre_rbt \<Rightarrow> 'a pre_rbt" where "LLR t \<equiv> LR (lsub t)"
-abbreviation LRL :: "'a pre_rbt \<Rightarrow> 'a pre_rbt" where "LRL t \<equiv> RL (lsub t)"
-abbreviation LRR :: "'a pre_rbt \<Rightarrow> 'a pre_rbt" where "LRR t \<equiv> RR (lsub t)"
-abbreviation RLL :: "'a pre_rbt \<Rightarrow> 'a pre_rbt" where "RLL t \<equiv> LL (rsub t)"
-abbreviation RLR :: "'a pre_rbt \<Rightarrow> 'a pre_rbt" where "RLR t \<equiv> LR (rsub t)"
-abbreviation RRL :: "'a pre_rbt \<Rightarrow> 'a pre_rbt" where "RRL t \<equiv> RL (rsub t)"
-abbreviation RRR :: "'a pre_rbt \<Rightarrow> 'a pre_rbt" where "RRR t \<equiv> RR (rsub t)"
-abbreviation LV :: "'a pre_rbt \<Rightarrow> 'a" where "LV t \<equiv> nval (lsub t)"
-abbreviation RV :: "'a pre_rbt \<Rightarrow> 'a" where "RV t \<equiv> nval (rsub t)"
-abbreviation LLV :: "'a pre_rbt \<Rightarrow> 'a" where "LLV t \<equiv> nval (LL t)"
-abbreviation LRV :: "'a pre_rbt \<Rightarrow> 'a" where "LRV t \<equiv> nval (LR t)"
-abbreviation RLV :: "'a pre_rbt \<Rightarrow> 'a" where "RLV t \<equiv> nval (RL t)"
-abbreviation RRV :: "'a pre_rbt \<Rightarrow> 'a" where "RRV t \<equiv> nval (RR t)"
+theorem pre_rbt_induct': "P Leaf \<Longrightarrow> (\<forall>t. P (lsub t) \<and> P (rsub t) \<longrightarrow> P t) \<Longrightarrow> P t"
+  apply (induction t) apply blast by (metis pre_rbt.sel(1) pre_rbt.sel(5))
+setup {* add_prfstep_induction @{thm pre_rbt_induct'} *}
 
-(* Some trivial lemmas. *)
+subsection {* Some trivial lemmas *}
+
 theorem not_R: "c \<noteq> R \<Longrightarrow> c = B" using color.exhaust by blast
 theorem not_B: "c \<noteq> B \<Longrightarrow> c = R" using color.exhaust by blast
 theorem red_not_leaf: "cl t = R \<Longrightarrow> t \<noteq> Leaf" by auto
@@ -51,58 +41,55 @@ theorem if_not_Leaf: "(if Node l c v r = Leaf then a else b) = b" by simp
 theorem if_R: "(if R = B then a else b) = b" by simp
 theorem if_B: "(if B = R then a else b) = b" by simp
 setup {* fold add_forward_prfstep [@{thm not_R}, @{thm not_B}, @{thm red_not_leaf}] *}
-setup {* fold add_simp_rule [@{thm if_not_Leaf}, @{thm if_R}, @{thm if_B}] *}
+setup {* fold add_rewrite_rule [@{thm if_not_Leaf}, @{thm if_R}, @{thm if_B}] *}
 
-(* Induction. *)
-theorem pre_rbt_induct': "P Leaf \<Longrightarrow> (\<forall>t. P (lsub t) \<and> P (rsub t) \<longrightarrow> P t) \<Longrightarrow> P t"
-  apply (induction t) apply blast by (metis pre_rbt.sel(1) pre_rbt.sel(5))
-setup {* add_prfstep_induction @{thm pre_rbt_induct'} *}
+section {* Definition of main functions and invariants *}
 
-(* Definition of main functions and invariants. *)
 fun min_depth :: "'a pre_rbt \<Rightarrow> nat" where
   "min_depth Leaf = 0"
 | "min_depth (Node l c a r) = min (min_depth l) (min_depth r) + 1"
-setup {* fold add_rewrite_rule @{thms min_depth.simps} *}
 
 fun max_depth :: "'a pre_rbt \<Rightarrow> nat" where
   "max_depth Leaf = 0"
 | "max_depth (Node l c a r) = max (max_depth l) (max_depth r) + 1"
-setup {* fold add_rewrite_rule @{thms max_depth.simps} *}
 
 fun black_depth :: "'a pre_rbt \<Rightarrow> nat" where
   "black_depth Leaf = 0"
-| "black_depth (Node l c a r) =
-    (if c = R then min (black_depth l) (black_depth r)
-     else min (black_depth l) (black_depth r) + 1)"
-setup {* fold add_rewrite_rule @{thms black_depth.simps} *}
+| "black_depth (Node l R a r) = min (black_depth l) (black_depth r)"
+| "black_depth (Node l B a r) = min (black_depth l) (black_depth r) + 1"
 
 fun cl_inv :: "'a pre_rbt \<Rightarrow> bool" where
   "cl_inv Leaf = True"
-| "cl_inv (Node l c a r) = (cl_inv l \<and> cl_inv r \<and> (if c = R then cl l = B \<and> cl r = B else True))"
-setup {* fold add_rewrite_rule @{thms cl_inv.simps} *}
+| "cl_inv (Node l R a r) = (cl_inv l \<and> cl_inv r \<and> cl l = B \<and> cl r = B)"
+| "cl_inv (Node l B a r) = (cl_inv l \<and> cl_inv r)"
 
 fun bd_inv :: "'a pre_rbt \<Rightarrow> bool" where
   "bd_inv Leaf = True"
 | "bd_inv (Node l c a r) = (bd_inv l \<and> bd_inv r \<and> black_depth l = black_depth r)"
-setup {* fold add_rewrite_rule @{thms bd_inv.simps} *}
 
 definition is_rbt :: "'a pre_rbt \<Rightarrow> bool" where
   "is_rbt t = (cl_inv t \<and> bd_inv t)"
-setup {* add_rewrite_rule @{thm is_rbt_def} *}
 
-(* More on bd_inv. *)
-theorem bd_inv_elim': "bd_inv (Node l c a r) \<Longrightarrow> black_depth (Node l c a r) =
-    (if c = R then black_depth l else black_depth l + 1)" by auto2
-theorem bd_inv_intro: "black_depth l = black_depth r \<Longrightarrow> (bd_inv l \<longrightarrow> bd_inv r \<longrightarrow> bd_inv (Node l c a r))" by auto2
+setup {* fold add_rewrite_rule (
+  @{thms min_depth.simps} @ @{thms max_depth.simps} @ @{thms black_depth.simps} @
+  @{thms cl_inv.simps} @ @{thms bd_inv.simps} @ [@{thm is_rbt_def}]) *}
 
-setup {* add_forward_prfstep @{thm bd_inv_elim'} *}
+subsection {* Properties of bd_inv *}
+
+theorem bd_inv_elimR: "bd_inv (Node l R a r) \<Longrightarrow> black_depth (Node l R a r) = black_depth l" by auto2
+theorem bd_inv_elimB: "bd_inv (Node l B a r) \<Longrightarrow> black_depth (Node l B a r) = black_depth l + 1" by auto2
+theorem bd_inv_intro: "black_depth l = black_depth r \<Longrightarrow> bd_inv l \<Longrightarrow> bd_inv r \<Longrightarrow> bd_inv (Node l c a r)" by auto2
+setup {* fold add_rewrite_rule [@{thm bd_inv_elimR}, @{thm bd_inv_elimB}] *}
 setup {* add_forward_prfstep_cond @{thm bd_inv_intro} [with_term "Node ?l ?c ?a ?r"] *}
 
-(* is_rbt is recursive. *)
-theorem is_rbt_rec: "is_rbt (Node l c a r) \<Longrightarrow> is_rbt l \<and> is_rbt r" by auto2
+subsection {* is_rbt is recursive *}
+
+theorem is_rbt_rec: "is_rbt (Node l c a r) \<Longrightarrow> is_rbt l \<and> is_rbt r"
+  by (tactic {* auto2s_tac @{context} (CASE "c = R") *})
 setup {* add_forward_prfstep @{thm is_rbt_rec} *}
 
-(* is_rbt condition implies that the tree is roughly balanced. *)
+section {* Balancedness of is_rbt *}
+
 theorem depth_min: "is_rbt t \<Longrightarrow> black_depth t \<le> min_depth t"
   by (tactic {* auto2s_tac @{context}
     (CASE "t = Leaf" THEN
@@ -123,104 +110,129 @@ theorem balanced: "is_rbt t \<Longrightarrow> max_depth t \<le> 2 * min_depth t 
      THEN OBTAIN "2 * black_depth t + 1 \<le> 2 * min_depth t + 1") *})
 setup {* fold del_prfstep_thm [@{thm depth_min}, @{thm depth_max}] *}
 
-(* Balance function. *)
-definition balanceR :: "'a pre_rbt \<Rightarrow> 'a pre_rbt" where
-  "balanceR t =
-    (if t = Leaf then Leaf else
-     if cl t = B then
-       if cl (rsub t) = R then
-         if cl (RL t) = R then
-           Node (Node (lsub t) B (nval t) (RLL t)) R (RLV t) (Node (RLR t) B (RV t) (RR t))
-         else if cl (RR t) = R then
-           Node (Node (lsub t) B (nval t) (RL t)) R (RV t) (Node (RRL t) B (RRV t) (RRR t))
-         else t
-       else t
-     else t)"
-definition balance :: "'a pre_rbt \<Rightarrow> 'a pre_rbt" where
-  "balance t =
-    (if t = Leaf then Leaf else
-     if cl t = B then
-       if cl (lsub t) = R then
-         if cl (LL t) = R then
-           Node (Node (LLL t) B (LLV t) (LLR t)) R (LV t) (Node (LR t) B (nval t) (rsub t))
-         else if cl (LR t) = R then
-           Node (Node (LL t) B (LV t) (LRL t)) R (LRV t) (Node (LRR t) B (nval t) (rsub t))
-         else balanceR t
-       else balanceR t
-     else t)"
-theorem balance_on_R: "balance (Node l R a r) = Node l R a r" by (simp add: balance_def)
+section {* Balancing function on RBT *}
 
-setup {*
-  add_rewrite_rule_cond @{thm balance_def} (with_conds ["?t \<noteq> lsub ?s", "?t \<noteq> rsub ?s"]) #>
-  add_rewrite_rule_cond @{thm balanceR_def} (with_conds ["?t \<noteq> lsub ?s", "?t \<noteq> rsub ?s"]) #>
-  add_rewrite_rule @{thm balance_on_R} *}
+fun balanceR :: "'a pre_rbt \<Rightarrow> 'a pre_rbt" where
+  "balanceR (Node a B x (Node (Node b R z c) R y d)) = Node (Node a B x b) R z (Node c B y d)"
+| "balanceR (Node a B x (Node b R y (Node c R z d))) = Node (Node a B x b) R y (Node c B z d)"
+| "balanceR t = t"
 
-(* Case checking when proving theorems involving balanceR t / balance t. *)
+theorem balanceR_def':
+  "cl b = B \<Longrightarrow> balanceR (Node a B x (Node b R y (Node c R z d))) = Node (Node a B x b) R y (Node c B z d)"
+  "cl r = B \<Longrightarrow> balanceR (Node l B x r) = Node l B x r"
+  "cl r = R \<Longrightarrow> cl (lsub r) = B \<Longrightarrow> cl (rsub r) = B \<Longrightarrow> balanceR (Node l B x r) = Node l B x r"
+apply (metis balanceR.simps(2) balanceR.simps(3) pre_rbt.collapse)
+apply (metis balanceR.simps(15) balanceR.simps(6) pre_rbt.collapse)
+by (smt balanceR.simps(10) balanceR.simps(13) balanceR.simps(14) balanceR.simps(9) pre_rbt.collapse red_not_leaf)
+setup {* fold add_rewrite_rule (@{thms balanceR.simps(1,4-5)} @ @{thms balanceR_def'}) *}
+
+fun balance :: "'a pre_rbt \<Rightarrow> 'a pre_rbt" where
+  "balance (Node (Node (Node a R z b) R y c) B x d) = Node (Node a B z b) R y (Node c B x d)"
+| "balance (Node (Node a R y (Node b R z c)) B x d) = Node (Node a B y b) R z (Node c B x d)"
+| "balance t = balanceR t"
+
+theorem balance_def':
+  "balance (Node l R x r) = Node l R x r"
+  "cl a = B \<Longrightarrow> balance (Node (Node a R y (Node b R z c)) B x d) = Node (Node a B y b) R z (Node c B x d)"
+  "cl l = B \<Longrightarrow> balance (Node l B x r) = balanceR (Node l B x r)"
+  "cl l = R \<Longrightarrow> cl (lsub l) = B \<Longrightarrow> cl (rsub l) = B \<Longrightarrow> balance (Node l B x r) = balanceR (Node l B x r)"
+apply simp apply (metis balance.simps(2) balance.simps(3) pre_rbt.collapse)
+apply (metis balance.simps(14) balance.simps(5) pre_rbt.collapse)
+by (smt balance.simps(11) balance.simps(12) balance.simps(4) balance.simps(7) balance.simps(8) pre_rbt.collapse red_not_leaf)
+setup {* fold add_rewrite_rule (@{thms balance.simps(1,4)} @ @{thms balance_def'}) *}
+
+text {*
+  Script specifying the case checking needed when proving theorems involving
+  balanceR t / balance t.
+*}
+
 ML {*
-val balanceR_scrpt =
+(* For balanceR t *)
+val balanceR_cases =
 CASE "t = Leaf"
 THEN CASE "cl t = B" WITH
   CASE "cl (rsub t) = R" WITH
-    (CASE "cl (RL t) = R" THEN CASE "cl (RR t) = R")
+    (CASE "cl (lsub (rsub t)) = R" THEN CASE "cl (rsub (rsub t)) = R")
 
-val balance_scrpt =
+(* For balance t *)
+val balance_cases =
 CASE "t = Leaf"
 THEN CASE "cl t = B" WITH
   CASE "cl (lsub t) = R" WITH
-    (CASE "cl (LL t) = R" THEN CASE "cl (LR t) = R")
+    (CASE "cl (lsub (lsub t)) = R" THEN CASE "cl (rsub (lsub t)) = R")
+
+(* For balanceR (Node l B x r) *)
+val balanceR_node_cases =
+  CASE "cl r = R" WITH (CASE "cl (lsub r) = R" THEN CASE "cl (rsub r) = R")
+
+(* For balance (Node l B x r) *)
+val balance_node_cases =
+  CASE "cl l = R" WITH (CASE "cl (lsub l) = R" THEN CASE "cl (rsub l) = R")
 *}
 
-(* Present function on RBT. Balance function preserves present. *)
-fun present :: "'a pre_rbt \<Rightarrow> 'a \<Rightarrow> bool" where
-  "present Leaf x = False"
-| "present (Node l c y r) x = (present l x \<or> x = y \<or> present r x)"
-setup {* fold add_rewrite_rule @{thms present.simps} *}
+subsection {* Balance function preserves set of keys *}
 
-theorem present_balanceR: "present (balanceR t) y = present t y"
-  by (tactic {* auto2s_tac @{context} balanceR_scrpt *})
-setup {* add_rewrite_rule @{thm present_balanceR} *}
-theorem present_balance: "present (balance t) y = present t y"
-  by (tactic {* auto2s_tac @{context} balance_scrpt *})
-setup {* add_rewrite_rule @{thm present_balance} *}
+fun rbt_set :: "'a pre_rbt \<Rightarrow> 'a set" where
+  "rbt_set Leaf = {}"
+| "rbt_set (Node l c y r) = {y} \<union> rbt_set l \<union> rbt_set r"
+setup {* fold add_rewrite_rule @{thms rbt_set.simps} *}
 
-(* balance function preserves bd_inv. *)
+theorem rbt_set_balanceR: "rbt_set (balanceR t) = rbt_set t"
+  by (tactic {* auto2s_tac @{context} balanceR_cases *})
+setup {* add_rewrite_rule @{thm rbt_set_balanceR} *}
+theorem rbt_set_balance: "rbt_set (balance t) = rbt_set t"
+  by (tactic {* auto2s_tac @{context} balance_cases *})
+setup {* add_rewrite_rule @{thm rbt_set_balance} *}
+
+subsection {* balance function preserves bd_inv *}
+
 theorem balance_bd': "bd_inv t \<Longrightarrow> bd_inv (balanceR t) \<and> black_depth t = black_depth (balanceR t)"
-  by (tactic {* auto2s_tac @{context} balanceR_scrpt *})
+  by (tactic {* auto2s_tac @{context} balanceR_cases *})
 setup {* fold add_backward_prfstep [conj_left_th @{thm balance_bd'}, conj_right_th @{thm balance_bd'}] *}
 
-theorem balance_bd: "bd_inv t \<Longrightarrow> bd_inv (balance t) \<and> black_depth t = black_depth (balance t)"
-  by (tactic {* auto2s_tac @{context} balance_scrpt *})
-setup {* add_backward_prfstep (conj_left_th @{thm balance_bd}) #>
-         add_forward_prfstep_cond (conj_right_th @{thm balance_bd}) [with_term "black_depth (balance ?t)"] *}
+theorem balance_bd: "bd_inv t \<Longrightarrow> bd_inv (balance t) \<and> black_depth (balance t) = black_depth t"
+  by (tactic {* auto2s_tac @{context} balance_cases *})
+setup {* add_backward_prfstep (conj_left_th @{thm balance_bd}) #> add_rewrite_rule (conj_right_th @{thm balance_bd}) *}
 
-(* cl_inv', and some trivial lemmas. *)
+subsection {* Definition and basic properties of cl_inv' *}
+
 fun cl_inv' :: "'a pre_rbt \<Rightarrow> bool" where
   "cl_inv' Leaf = True"
 | "cl_inv' (Node l c a r) = (cl_inv l \<and> cl_inv r)"
+setup {* fold add_rewrite_rule @{thms cl_inv'.simps} *}
 
-theorem cl_inv_def': "cl_inv (Node l c a r) \<Longrightarrow> cl_inv l \<and> cl_inv r" by simp
-theorem cl_inv_def1: "cl_inv (Node l B a r) = (cl_inv l \<and> cl_inv r)" by simp
-theorem cl_inv_def2: "cl_inv (Node l R a r) = (cl_inv l \<and> cl_inv r \<and> cl l = B \<and> cl r = B)" by simp
-setup {* fold add_rewrite_rule (@{thms cl_inv'.simps} @ [@{thm cl_inv_def1}, @{thm cl_inv_def2}]) *}
-setup {* add_forward_prfstep @{thm cl_inv_def'} *}
-setup {* del_prfstep_thm @{thm cl_inv.simps(2)} *}
+theorem cl_inv_B: "cl t = B \<Longrightarrow> cl_inv' t \<Longrightarrow> cl_inv t" by auto2
+theorem cl_inv_R: "cl_inv' (Node l R x r) \<Longrightarrow> cl l = B \<Longrightarrow> cl r = B \<Longrightarrow> cl_inv (Node l R x r)" by auto2
+theorem cl_inv_imp: "cl_inv t \<Longrightarrow> cl_inv' t" by (tactic {* auto2s_tac @{context} (CASE "cl t = R") *})
+setup {* add_backward2_prfstep @{thm cl_inv_B} #> add_forward_prfstep @{thm cl_inv_imp} *}
+setup {* fold add_forward_prfstep [@{thm cl_inv_B}, @{thm cl_inv_R}] *}
 
-theorem cl_inv_B: "cl_inv' t \<Longrightarrow> cl t = B \<Longrightarrow> cl_inv t" by auto2
-theorem cl_inv_imp: "cl_inv t \<Longrightarrow> cl_inv' t" by auto2
-setup {* add_backward1_prfstep @{thm cl_inv_B} #> add_resolve_prfstep @{thm cl_inv_imp} *}
+subsection {* balance function preserves cl_inv *}
 
-(* balance function preserves cl_inv. *)
-theorem balanceR: "cl_inv l \<Longrightarrow> cl_inv' r \<Longrightarrow> cl_inv (balanceR (Node l B a r))" by auto2
+theorem balanceR: "cl_inv l \<Longrightarrow> cl_inv' r \<Longrightarrow> cl_inv (balanceR (Node l B a r))"
+  by (tactic {* auto2s_tac @{context} balanceR_node_cases *})
 setup {* add_backward1_prfstep @{thm balanceR} #> add_backward2_prfstep @{thm balanceR} *}
 
-theorem balance1: "cl_inv' l \<Longrightarrow> cl_inv r \<Longrightarrow> cl_inv (balance (Node l B a r))" by auto2
-theorem balance2: "cl_inv l \<Longrightarrow> cl_inv' r \<Longrightarrow> cl_inv (balance (Node l B a r))" by auto2
+theorem balance1: "cl_inv' l \<Longrightarrow> cl_inv r \<Longrightarrow> cl_inv (balance (Node l B a r))"
+  by (tactic {* auto2s_tac @{context} balance_node_cases *})
+theorem balance2: "cl_inv l \<Longrightarrow> cl_inv' r \<Longrightarrow> cl_inv (balance (Node l B a r))"
+  by (tactic {* auto2s_tac @{context} balance_node_cases *})
 setup {* del_prfstep_thm @{thm balanceR} *}
 setup {* fold (fn th => add_backward1_prfstep th o add_backward2_prfstep th)
               [@{thm balance1}, @{thm balance2}] *}
 
-(* Insert function. *)
-fun ins :: "nat \<Rightarrow> nat pre_rbt \<Rightarrow> nat pre_rbt" where
+subsection {* Balance function takes non-leafs to non-leafs *}
+
+theorem balanceR_non_Leaf: "balanceR (Node l c a r) \<noteq> Leaf"
+  by (tactic {* auto2s_tac @{context} (CASE "c = R" THEN balanceR_node_cases) *})
+setup {* add_resolve_prfstep @{thm balanceR_non_Leaf} *}
+theorem balance_non_Leaf: "balance (Node l c a r) \<noteq> Leaf"
+  by (tactic {* auto2s_tac @{context} (CASE "c = R" THEN balance_node_cases) *})
+setup {* add_forward_prfstep_cond @{thm balance_non_Leaf} [with_term "balance (Node ?l ?c ?a ?r)"] *}
+
+section {* ins function *}
+
+fun ins :: "'a::order \<Rightarrow> 'a pre_rbt \<Rightarrow> 'a pre_rbt" where
   "ins x Leaf = Node Leaf R x Leaf"
 | "ins x (Node l c y r) =
     (if x = y then Node l c y r
@@ -228,13 +240,12 @@ fun ins :: "nat \<Rightarrow> nat pre_rbt \<Rightarrow> nat pre_rbt" where
      else balance (Node l c y (ins x r)))"
 setup {* fold add_rewrite_rule @{thms ins.simps} *}
 
-theorem balanceR_non_Leaf: "balanceR (Node l c a r) \<noteq> Leaf" by auto2
-setup {* add_resolve_prfstep @{thm balanceR_non_Leaf} *}
-theorem balance_non_Leaf: "balance (Node l c a r) \<noteq> Leaf" by auto2
-setup {* add_forward_prfstep_cond @{thm balance_non_Leaf} [with_term "balance (Node ?l ?c ?a ?r)"] *}
+subsection {* ins function takes non-leaf to non-leafs *}
 
 theorem ins_non_Leaf: "ins x t \<noteq> Leaf" by auto2
 setup {* add_forward_prfstep_cond @{thm ins_non_Leaf} [with_term "ins ?x ?t"] *}
+
+subsection {* Properties of ins function on cl_inv, bd_inv, and set of keys *}
 
 theorem cl_inv_ins: "cl_inv t \<Longrightarrow> if cl t = B then cl_inv (ins x t) else cl (ins x t) = R \<and> cl_inv' (ins x t)" by auto2
 
@@ -244,22 +255,25 @@ theorem cl_inv_ins_r: "cl_inv t \<Longrightarrow> cl_inv (rsub (ins x t))" by au
 setup {* del_prfstep_thm @{thm cl_inv_ins} *}
 setup {* fold add_backward_prfstep [@{thm cl_inv_ins_l}, @{thm cl_inv_ins_r}] *}
 
-theorem bd_inv_ins: "bd_inv t \<Longrightarrow> bd_inv (ins x t) \<and> black_depth t = black_depth (ins x t)" by auto2
+theorem bd_inv_ins: "bd_inv t \<Longrightarrow> bd_inv (ins x t) \<and> black_depth t = black_depth (ins x t)"
+  by (tactic {* auto2s_tac @{context} (CASE "cl t = R") *})
 setup {* add_forward_prfstep_cond (conj_left_th @{thm bd_inv_ins}) [with_term "ins ?x ?t"] *}
 
-theorem present_ins: "present (ins x t) y = (x = y \<or> present t y)" by auto2
-setup {* add_rewrite_rule @{thm present_ins} *}
+theorem rbt_set_ins: "rbt_set (ins x t) = {x} \<union> rbt_set t" by auto2
+setup {* add_rewrite_rule @{thm rbt_set_ins} *}
+
+section {* Insert function *}
 
 fun makeBlack :: "'a pre_rbt \<Rightarrow> 'a pre_rbt" where
   "makeBlack Leaf = Leaf"
 | "makeBlack (Node l c a r) = Node l B a r"
-definition rbt_insert :: "nat \<Rightarrow> nat pre_rbt \<Rightarrow> nat pre_rbt" where
+definition rbt_insert :: "'a::order \<Rightarrow> 'a pre_rbt \<Rightarrow> 'a pre_rbt" where
   "rbt_insert x t = makeBlack (ins x t)"
 
 setup {* fold add_rewrite_rule (@{thms makeBlack.simps} @ [@{thm rbt_insert_def}]) *}
 
-theorem present_makeBlack: "present (makeBlack t) y = present t y" by auto2
-setup {* add_rewrite_rule @{thm present_makeBlack} *}
+theorem rbt_set_makeBlack: "rbt_set (makeBlack t) = rbt_set t" by auto2
+setup {* add_rewrite_rule @{thm rbt_set_makeBlack} *}
 
 theorem cl_inv_insert: "cl_inv t \<Longrightarrow> cl_inv (rbt_insert x t)" by auto2
 theorem bd_inv_insert: "bd_inv t \<Longrightarrow> bd_inv (rbt_insert x t)" by auto2
@@ -267,58 +281,39 @@ setup {* fold add_backward_prfstep [@{thm cl_inv_insert}, @{thm bd_inv_insert}] 
 
 theorem is_rbt_insert: "is_rbt t \<Longrightarrow> is_rbt (rbt_insert x t)" by auto2
 
-theorem present_insert: "present (rbt_insert x t) y = (x = y \<or> present t y)" by auto2
+theorem rbt_set_insert: "rbt_set (rbt_insert x t) = {x} \<union> rbt_set t" by auto2
 
-(* Sortedness on trees. *)
+section {* Sortedness on trees *}
+
 fun base_tree :: "'a pre_rbt \<Rightarrow> 'a tree" where
   "base_tree Leaf = Tip"
 | "base_tree (Node l c a r) = Lists_Ex.Node (base_tree l) a (base_tree r)"
 setup {* fold add_rewrite_rule @{thms base_tree.simps} *}
 
-theorem balanceR_as_rotate: "base_tree (balanceR t) =
-  (if t = Leaf then Tip else
-   if cl t = B then
-     if cl (rsub t) = R then
-       if cl (RL t) = R then rotateL (rotateR_at_R (base_tree t))
-       else if cl (RR t) = R then rotateL (base_tree t)
-       else base_tree t
-     else base_tree t
-   else base_tree t)"
-  by (tactic {* auto2s_tac @{context} balanceR_scrpt *})
+theorem balanceR_as_rotate1: "cl r = R \<Longrightarrow> cl (lsub r) = R \<Longrightarrow>
+  base_tree (balanceR (Node l B x r)) = rotateL (rotateR_at_R (base_tree (Node l B x r)))" by auto2
+theorem balanceR_as_rotate2: "cl r = R \<Longrightarrow> cl (lsub r) = B \<Longrightarrow> cl (rsub r) = R \<Longrightarrow>
+  base_tree (balanceR (Node l B x r)) = rotateL (base_tree (Node l B x r))" by auto2
+theorem balance_as_rotate1: "cl l = R \<Longrightarrow> cl (lsub l) = R \<Longrightarrow>
+  base_tree (balance (Node l B x r)) = rotateR (base_tree (Node l B x r))" by auto2
+theorem balance_as_rotate2: "cl l = R \<Longrightarrow> cl (lsub l) = B \<Longrightarrow> cl (rsub l) = R \<Longrightarrow>
+  base_tree (balance (Node l B x r)) = rotateR (rotateL_at_L (base_tree (Node l B x r)))" by auto2
+setup {* fold add_rewrite_rule [@{thm balanceR_as_rotate1}, @{thm balanceR_as_rotate2},
+  @{thm balance_as_rotate1}, @{thm balance_as_rotate2}] *}
 
-theorem balance_as_rotate: "base_tree (balance t) =
-  (if t = Leaf then Tip else
-   if cl t = B then
-     if cl (lsub t) = R then
-       if cl (LL t) = R then rotateR (base_tree t)
-       else if cl (LR t) = R then rotateR (rotateL_at_L (base_tree t))
-       else base_tree (balanceR t)
-     else base_tree (balanceR t)
-   else base_tree t)"
-  by (tactic {* auto2s_tac @{context} balance_scrpt *})
-
-setup {* fold add_rewrite_rule [@{thm balanceR_as_rotate}, @{thm balance_as_rotate}] *}
-
-definition rbt_sorted :: "nat pre_rbt \<Rightarrow> bool" where
+definition rbt_sorted :: "'a::linorder pre_rbt \<Rightarrow> bool" where
   "rbt_sorted t = tree_sorted (base_tree t)"
 setup {* add_rewrite_rule_bidir @{thm rbt_sorted_def} *}
 
-theorem rbt_present: "present t x = tree_present (base_tree t) x" by auto2
-setup {* add_rewrite_rule_bidir @{thm rbt_present} *}
+theorem rbt_set_base: "rbt_set t = tree_set (base_tree t)" by auto2
+setup {* add_rewrite_rule_bidir @{thm rbt_set_base} *}
 
 theorem balanceR_sorted: "rbt_sorted t \<Longrightarrow> rbt_sorted (balanceR t)"
-  by (tactic {* auto2s_tac @{context} balanceR_scrpt *})
+  by (tactic {* auto2s_tac @{context} balanceR_cases *})
 setup {* add_backward_prfstep @{thm balanceR_sorted} *}
-
 theorem balance_sorted: "rbt_sorted t \<Longrightarrow> rbt_sorted (balance t)"
-  by (tactic {* auto2s_tac @{context} balance_scrpt *})
+  by (tactic {* auto2s_tac @{context} balance_cases *})
 setup {* add_backward_prfstep @{thm balance_sorted} *}
-
-theorem rbt_sorted_def': "rbt_sorted (Node l c a r) =
-  ((\<forall>x. present l x \<longrightarrow> x < a) \<and> (\<forall>x. present r x \<longrightarrow> a < x) \<and>
-   rbt_sorted l \<and> rbt_sorted r)" by auto2
-setup {* add_rewrite_rule @{thm rbt_sorted_def'} *}
-setup {* del_prfstep_thm @{thm rbt_sorted_def} *}
 
 theorem ins_sorted: "rbt_sorted t \<Longrightarrow> rbt_sorted (ins x t)"
   by (tactic {* auto2s_tac @{context}
@@ -329,8 +324,9 @@ theorem insert_sorted: "rbt_sorted t \<Longrightarrow> rbt_sorted (rbt_insert x 
   by (tactic {* auto2s_tac @{context}
     (OBTAIN "rbt_sorted (ins x t) = rbt_sorted (rbt_insert x t)") *})
 
-(* Search on sorted trees and its correctness. *)
-fun rbt_search :: "nat pre_rbt \<Rightarrow> nat \<Rightarrow> bool" where
+section {* Search on sorted trees and its correctness *}
+
+fun rbt_search :: "'a::ord pre_rbt \<Rightarrow> 'a \<Rightarrow> bool" where
   "rbt_search Leaf x = False"
 | "rbt_search (Node l c y r) x =
   (if x = y then True
@@ -338,6 +334,6 @@ fun rbt_search :: "nat pre_rbt \<Rightarrow> nat \<Rightarrow> bool" where
    else rbt_search r x)"
 setup {* fold add_rewrite_rule @{thms rbt_search.simps} *}
 
-theorem rbt_search_correct: "rbt_sorted t \<Longrightarrow> (rbt_search t x = present t x)" by auto2
+theorem rbt_search_correct: "rbt_sorted t \<Longrightarrow> (rbt_search t x \<longleftrightarrow> x \<in> rbt_set t)" by auto2
 
 end
