Auto2_Base.thy
@@ -7,13 +7,19 @@ ML_file "box_id.ML"
 ML_file "acdata.ML"
 ML_file "subterms.ML"
 ML_file "rewrite.ML"
-ML_file "normalize.ML"
 ML_file "status.ML"
+ML_file "normalize.ML"
 ML_file "proofsteps.ML"
 ML_file "script.ML"
 ML_file "auto2.ML"
 ML_file "induction.ML"
 
 method_setup auto2 = {* Scan.succeed (SIMPLE_METHOD o auto2_tac) *} "auto2 prover"
+
+text {* First add proofstep converting any PROP equality to EQ. Then use EQ to match
+  equality in all proofsteps. *}
+theorem trivial_eq: "A = B \<Longrightarrow> A = B" by simp
+setup {* add_forward_prfstep @{thm trivial_eq} #>
+  ItemIO_Data.add_item_to_th (ItemIO_Data.eq_prop_filt, ItemIO_Data.eq_prop_match) *}
 
 end
