Auto2_Test.thy
@@ -3,6 +3,7 @@ imports Auto2
 begin
 
 ML_file "logic_steps_test.ML"
+ML_file "order_test.ML"
 
 setup {* clear_ac_data *}
 
