Imp_Ex_Quicksort.thy
@@ -1,0 +1,187 @@
+theory Imp_Ex_Quicksort
+imports Imp_Thms
+begin
+
+fun swap :: "'a\<Colon>heap array \<Rightarrow> nat \<Rightarrow> nat \<Rightarrow> unit Heap" where
+  "swap a i j = do {
+     x \<leftarrow> Array.nth a i;
+     y \<leftarrow> Array.nth a j;
+     Array.upd i y a;
+     Array.upd j x a;
+     return ()
+   }"
+
+function part1 :: "nat array \<Rightarrow> nat \<Rightarrow> nat \<Rightarrow> nat \<Rightarrow> nat Heap"
+where
+  "part1 a left right p = (
+     if (right \<le> left) then return right
+     else do {
+       v \<leftarrow> Array.nth a left;
+       (if v \<le> p
+        then (part1 a (left + 1) right p)
+        else (do { swap a left right;
+                   part1 a left (right - 1) p }))
+     })"
+by pat_completeness auto termination by (relation "measure (\<lambda>(_,l,r,_). r - l )") auto
+
+(* Properties of swap. *)
+setup {* add_rewrite_rule @{thm swap.simps} *}
+lemma swap_pointwise: "effect (swap a i j) h h' r \<Longrightarrow>
+  Array.get h' a ! k = (if k = i then Array.get h a ! j else if k = j then Array.get h a ! i else Array.get h a ! k)" by auto2
+lemma swap_permutes: "effect (swap a i j) h h' rs \<Longrightarrow>
+  multiset_of (Array.get h' a) = multiset_of (Array.get h a)" by auto2
+lemma swap_length: "effect (swap a i j) h h' r \<Longrightarrow> Array.length h' a = Array.length h a" by auto2
+lemma swap_succeed: "i < Array.length h a \<and> j < Array.length h a \<Longrightarrow> success (swap a i j) h" by auto2
+setup {* del_prfstep_thm @{thm swap.simps}
+      #> fold add_rewrite_rule [@{thm swap_pointwise}, @{thm swap_permutes}, @{thm swap_length}]
+      #> add_backward_prfstep @{thm swap_succeed} *}
+
+(* Induction rule for part1. *)
+setup {* add_rewrite_rule_cond @{thm part1.simps} (with_filts [size1_filter "left", size1_filter "right"]) *}
+theorem part1_induct': "(\<forall>a left right p.
+    ((\<not> right \<le> left \<longrightarrow> (\<forall>v.  v \<le> p \<longrightarrow> P a (left + 1) right p)) \<and>
+     (\<not> right \<le> left \<longrightarrow> (\<forall>v. \<not>v \<le> p \<longrightarrow> P a left (right - 1) p))) \<longrightarrow> P a left right p) \<Longrightarrow>
+    P (a::nat array) (left::nat) (right::nat) (p::nat)"
+  apply (induct rule: part1.induct) by blast
+setup {* add_prfstep_imp_induction @{term_pat "part1 ?a ?l ?r ?p"} @{thm part1_induct'} *}
+
+(* Properties of part1. *)
+lemma part1_permutes: "effect (part1 a l r p) h h' rs \<Longrightarrow>
+  multiset_of (Array.get h' a) = multiset_of (Array.get h a)" by auto2
+setup {* add_rewrite_rule @{thm part1_permutes} *}
+
+lemma part1_returns_index_in_bounds': "effect (part1 a l r p) h h' rs \<Longrightarrow>
+  if r \<le> l then rs = r else l \<le> rs \<and> rs \<le> r" by auto2
+lemma part1_returns_index_in_bounds: "effect (part1 a l r p) h h' rs \<Longrightarrow>
+  l \<le> r \<Longrightarrow> l \<le> rs \<and> rs \<le> r" by (metis order_refl part1_returns_index_in_bounds')
+setup {* add_forward_prfstep @{thm part1_returns_index_in_bounds} *}
+
+lemma part1_outer_remains: "effect (part1 a l r p) h h' rs \<Longrightarrow> outer_remains h h' a l r" by auto2
+setup {* add_forward_prfstep @{thm part1_outer_remains} *}
+
+lemma part1_partitions1: "effect (part1 a l r p) h h' rs \<Longrightarrow> l \<le> i \<and> i < rs \<Longrightarrow> Array.get h' a ! i \<le> p" by auto2
+lemma part1_partitions2: "effect (part1 a l r p) h h' rs \<Longrightarrow> rs < i \<and> i \<le> r \<Longrightarrow> Array.get h' a ! i \<ge> p" by auto2
+setup {* fold add_backward2_prfstep [@{thm part1_partitions1}, @{thm part1_partitions2}] *}
+
+lemma part1_succeed: "l < Array.length h a \<and> r < Array.length h a \<Longrightarrow> success (part1 a l r p) h" by auto2
+setup {* add_backward_prfstep @{thm part1_succeed} *}
+
+setup {* fold del_prfstep_thm [@{thm part1.simps}, @{thm part1_induct'}] *}
+
+(* Partition function. *)
+fun partition :: "nat array \<Rightarrow> nat \<Rightarrow> nat \<Rightarrow> nat Heap"
+where
+  "partition a left right = do {
+     pivot \<leftarrow> Array.nth a right;
+     middle \<leftarrow> part1 a left (right - 1) pivot;
+     v \<leftarrow> Array.nth a middle;
+     m \<leftarrow> return (if (v \<le> pivot) then (middle + 1) else middle);
+     comment (\<lambda>h. (\<forall>i. left \<le> i \<and> i < m \<longrightarrow> Array.get h a ! i \<le> pivot) \<and>
+                  (\<forall>i. m \<le> i \<and> i < right - 1 \<longrightarrow> Array.get h a ! i \<ge> pivot) \<and>
+                  Array.get h a ! right = pivot);
+     swap a m right;
+     return m
+   }"
+
+(* Properties of partition. *)
+setup {* add_rewrite_rule @{thm partition.simps} *}
+lemma partition_succeed: "l < r \<and> r < Array.length h a \<Longrightarrow> success (partition a l r) h" by auto2
+setup {* add_backward_prfstep @{thm partition_succeed} *}
+
+lemma partition_permutes: "effect (partition a l r) h h' rs \<Longrightarrow>
+  multiset_of (Array.get h' a) = multiset_of (Array.get h a)" by auto2
+setup {* add_rewrite_rule @{thm partition_permutes} *}
+
+lemma partition_outer_remains: "effect (partition a l r) h h' rs \<Longrightarrow>
+  l < r \<Longrightarrow> outer_remains h h' a l r" by auto2
+setup {* add_forward_prfstep @{thm partition_outer_remains} *}
+
+lemma partition_returns_index_in_bounds: "effect (partition a l r) h h' rs \<Longrightarrow>
+  l < r \<Longrightarrow> l \<le> rs \<le> r" by auto2
+setup {* add_forward_prfstep @{thm partition_returns_index_in_bounds} *}
+
+lemma partition_partitions1: "effect (partition a l r) h h' rs \<Longrightarrow> l < r \<Longrightarrow>
+  (\<forall>x\<in>set (subarray l rs a h'). x \<le> Array.get h' a ! rs)" by auto2
+lemma partition_partitions2: "effect (partition a l r) h h' rs \<Longrightarrow> l < r \<Longrightarrow>
+  (\<forall>y\<in>set (subarray (rs + 1) (r + 1) a h'). Array.get h' a ! rs \<le> y)" by auto2
+setup {* del_prfstep_thm @{thm partition.simps}
+  #> fold add_forward_prfstep [@{thm partition_partitions1}, @{thm partition_partitions2}] *}
+
+(* Quicksort function *)
+function quicksort :: "nat array \<Rightarrow> nat \<Rightarrow> nat \<Rightarrow> unit Heap"
+where
+  "quicksort a left right =
+     (if left < right then
+        do {
+          pivot \<leftarrow> partition a left right;
+          pivot \<leftarrow> assert (\<lambda>x. left \<le> x \<and> x \<le> right) pivot;
+          comment (\<lambda>h. if pivot > 0 then pivot = 1 + (pivot - 1) else pivot = 0);
+          quicksort a left (pivot - 1);
+          quicksort a (pivot + 1) right
+        }
+     else return ())"
+by pat_completeness auto termination by (relation "measure (\<lambda>(a, l, r). (r - l))") auto
+
+(* Induction rule for quicksort. *)
+setup {* add_rewrite_rule_cond @{thm quicksort.simps} (with_filts [size1_filter "left", size1_filter "right"]) *}
+theorem quicksort_induct': "(\<forall>arr left right.
+    ((left < right \<longrightarrow> (\<forall>p. left \<le> p \<le> right \<longrightarrow> P arr left (p - 1))) \<and>
+     (left < right \<longrightarrow> (\<forall>p. left \<le> p \<le> right \<longrightarrow> P arr (p + 1) right))) \<longrightarrow> P arr left right) \<Longrightarrow>
+    P (arr::nat array) (left::nat) (right::nat)"
+  apply (induct rule: quicksort.induct) by (metis closed_interval_def)
+setup {* add_prfstep_imp_induction @{term_pat "quicksort ?a ?left ?right"} @{thm quicksort_induct'} *}
+
+lemma quicksort_outer_remains: "effect (quicksort a l r) h h' rs \<Longrightarrow> outer_remains h h' a l r" by auto2
+setup {* add_forward_prfstep @{thm quicksort_outer_remains} *}
+
+lemma quicksort_permutes: "effect (quicksort a l r) h h' rs \<Longrightarrow>
+  multiset_of (Array.get h' a) = multiset_of (Array.get h a)" by auto2
+setup {* add_forward_prfstep @{thm quicksort_permutes} *}
+
+theorem quicksort_permutes': "effect (quicksort a l r) h h' rs \<Longrightarrow>
+  r < Array.length h a \<Longrightarrow> multiset_of (subarray l (r + 1) a h) = multiset_of (subarray l (r + 1) a h')"
+  by (tactic {* auto2s_tac @{context} (OBTAIN "multiset_of (Array.get h' a) = multiset_of (Array.get h a)") *})
+setup {* del_prfstep_thm @{thm quicksort_permutes} #> add_forward_prfstep @{thm quicksort_permutes'} *}
+
+lemma quicksort_is_skip: "effect (quicksort a l r) h h' rs \<Longrightarrow> r \<le> l \<Longrightarrow> h' = h" by auto2
+setup {* add_forward_prfstep @{thm quicksort_is_skip} *}
+
+lemma quicksort_success_skip: "\<not>r > l \<Longrightarrow> success (quicksort a l r) h" by auto2
+setup {* add_backward_prfstep @{thm quicksort_success_skip} *}
+
+lemma quicksort_success: "l < Array.length h a \<and> r < Array.length h a \<Longrightarrow>
+  success (quicksort a l r) h" by auto2
+
+(* Now for the final theorem. *)
+setup {* add_gen_prfstep ("quicksort_case",
+  [WithFact @{term_pat "effect (quicksort ?a ?l ?r) ?h ?h' ?rs"},
+   CreateCase ([@{term_pat "(?l::nat) < ?r"}], [])]) *}
+
+(* Outer remains theorems particular to quicksort. *)
+theorem outer_remains_qs1: "outer_remains h h' a (l+1) r \<Longrightarrow>
+  Array.get h a ! l = Array.get h' a ! l \<and> subarray x l a h = subarray x l a h'" by auto2
+theorem outer_remains_qs2: "outer_remains h h' a l r \<Longrightarrow>
+  Array.get h a ! (r+1) = Array.get h' a ! (r+1) \<and> subarray (r+2) y a h = subarray (r+2) y a h'" by auto2
+setup {* fold (add_rewrite_rule o conj_left_th) [@{thm outer_remains_qs1}, @{thm outer_remains_qs2}] *}
+setup {* fold (add_rewrite_rule o conj_right_th) [@{thm outer_remains_qs1}, @{thm outer_remains_qs2}] *}
+
+(* Sortedness of lists of form x @ [pivot] @ y. *)
+setup {* add_rewrite_rule @{thm sorted_append} *}
+theorem sorted_pivoted_list: "sorted (sublist' l pivot xs) \<Longrightarrow> sorted (sublist' (pivot + 1) r xs) \<Longrightarrow>
+  \<forall>x\<in>set (sublist' l pivot xs). x \<le> xs ! pivot \<Longrightarrow> \<forall>y\<in>set (sublist' (pivot + 1) r xs). xs ! pivot \<le> y \<Longrightarrow>
+  l \<le> pivot \<Longrightarrow> pivot < r \<Longrightarrow> r \<le> length xs \<Longrightarrow> sorted (sublist' l r xs)"
+  by (tactic {* auto2s_tac @{context} (
+      OBTAIN "sublist' pivot r xs = xs ! pivot # sublist' (pivot + 1) r xs" THEN
+      CASE "pivot = 0" THEN OBTAIN "sublist' l r xs = sublist' l pivot xs @ sublist' pivot r xs") *})
+setup {* del_prfstep_thm @{thm sorted_append} #> add_forward_prfstep @{thm sorted_pivoted_list} *}
+
+theorem sorted_pivoted_list': "sorted (sublist' 1 r xs) \<Longrightarrow>
+  \<forall>y\<in>set (sublist' 1 r xs). xs ! 0 \<le> y \<Longrightarrow> r \<le> length xs \<Longrightarrow> sorted (sublist' 0 r xs)"
+  by (tactic {* auto2s_tac @{context} (OBTAIN "sublist' 0 r xs = xs ! 0 # sublist' 1 r xs") *})
+setup {* add_forward_prfstep @{thm sorted_pivoted_list'} *}
+
+lemma quicksort_sorts: "effect (quicksort a l r) h h' rs \<Longrightarrow>
+  l < Array.length h a \<Longrightarrow> r < Array.length h a \<Longrightarrow>
+  sorted (subarray l (r + 1) a h')" by auto2
+
+end
