Logic_Thms.thy
@@ -3,7 +3,7 @@ imports Auto2_Base
 begin
 
 setup {* fold add_rew_const [@{term "True"}, @{term "False"}] *}
-setup {* fold add_normalizer
+setup {* fold add_th_normalizer
   [("split_conj", K split_conj_th), ("split_not_disj", K split_not_disj_th)] *}
 
 (* AC-property of conj and disj. *)
@@ -11,87 +11,68 @@ theorem conj_true_neutral: "(True \<and> A) = A" by simp
 theorem disj_false_neutral: "(False \<or> A) = A" by simp
 ML {*
 val add_logic_ac_data =
-  add_ac_data {fname = @{const_name disj}, assoc_r = true,
-               unit_val = @{term False}, comm_th = @{thm disj_commute},
-               assoc_th = @{thm disj_assoc}, unit_th = @{thm disj_false_neutral}} #>
-  add_ac_data {fname = @{const_name conj}, assoc_r = true,
-               unit_val = @{term True}, comm_th = @{thm conj_commute},
-               assoc_th = @{thm conj_assoc}, unit_th = @{thm conj_true_neutral}}
+    fold add_ac_data [
+      {fname = @{const_name disj}, assoc_r = true,
+       unit_val = @{term False}, comm_th = @{thm disj_commute},
+       assoc_th = @{thm disj_assoc}, unit_th = @{thm disj_false_neutral}},
+
+      {fname = @{const_name conj}, assoc_r = true,
+       unit_val = @{term True}, comm_th = @{thm conj_commute},
+       assoc_th = @{thm conj_assoc}, unit_th = @{thm conj_true_neutral}}]
 *}
 setup {* add_logic_ac_data *}
 
 (* Rewrites A = True to A, etc. *)
-theorem simp_eq_True: "(A simp= True) = A" by (simp add: simp_eq_def)
-theorem simp_eq_False: "(A simp= False) = (\<not>A)" by (simp add: simp_eq_def)
 theorem neq_True: "(A \<noteq> True) = (\<not>A)" by simp
 theorem neq_False: "(A \<noteq> False) = A" by simp
 setup {* fold add_eq_th_normalizer
-  [@{thm HOL.eq_True}, @{thm HOL.eq_False}, @{thm simp_eq_True}, @{thm simp_eq_False},
-   @{thm neq_True}, @{thm neq_False}] *}
-theorem eq_False': "((\<not>A) = False) = A" by simp
+  [@{thm HOL.eq_True}, @{thm HOL.eq_False}, @{thm neq_True}, @{thm neq_False}] *}
 
 (* Trivial contradictions. *)
 setup {* add_resolve_prfstep @{thm HOL.refl} *}
-theorem imp_triv: "A \<Longrightarrow> A" by simp
-setup {* add_resolve_prfstep @{thm imp_triv} *}
+setup {* add_forward_prfstep @{thm contra_triv} *}
 
 (* Conj. Will be expanded by normalizer. *)
-setup {* add_prfstep (prfstep_custom "conj_fact_list"
-  [WithFact @{term_pat "?A \<and> ?B"},
-   Filter (canonical_split_filter @{const_name conj} "A" "B")]
-  (fn ((id, _), ths) => fn _ => [Update.thm_update (id, the_single ths)])) *}
+theorem conj_id: "A \<and> B \<Longrightarrow> A \<and> B" by simp
+setup {* add_forward_prfstep_cond @{thm conj_id}
+  [with_filt (canonical_split_filter @{const_name conj} "A" "B")] *}
 
 (* Disj. Will be expanded by normalizer. *)
-setup {* add_prfstep (prfstep_custom "disj_goal_list"
-  [WithGoal @{term_pat "?A \<or> ?B"},
-   Filter (canonical_split_filter @{const_name disj} "A" "B")]
-  (fn ((id, _), ths) => fn _ => [Update.thm_update (id, the_single ths)])) *}
-
-(* Equality. Invoke special treatment of equality. *)
-theorem eq_elim: "C = (A = B) \<Longrightarrow> C \<Longrightarrow> A = B" by simp
-setup {* add_forward_prfstep @{thm eq_elim} *}
+theorem disj_id: "A \<or> B \<Longrightarrow> A \<or> B" by simp
+setup {* add_backward_prfstep_cond @{thm disj_id}
+  [with_filt (canonical_split_filter @{const_name disj} "A" "B")] *}
 
 (* Not. *)
-ML {* val nn_cancel_th = @{thm HOL.nnf_simps(6)} *}
-setup {* add_simp_rule nn_cancel_th #> add_eq_th_normalizer nn_cancel_th *}
+setup {* add_rewrite_rule nn_cancel_th #> add_eq_th_normalizer nn_cancel_th *}
 
 (* Iff. *)
 setup {* add_gen_prfstep ("iff_intro1",
   [WithGoal @{term_pat "(?A::bool) = ?B"},
    CreateCase ([@{term_pat "?A::bool"}], [@{term_pat "?B::bool"}])]) *}
 setup {* add_fixed_sc ("iff_intro1", 25) *}  (* includes the cost of creating a case. *)
-theorem iff_intro2: "A \<longrightarrow> B \<Longrightarrow> \<not>(A = B) \<Longrightarrow> \<not>A \<and> B" by simp
+theorem iff_intro2: "A \<longrightarrow> B \<Longrightarrow> \<not>(A \<longleftrightarrow> B) \<Longrightarrow> \<not>A \<and> B" by simp
 setup {* add_forward_prfstep @{thm iff_intro2} *}
 setup {* add_fixed_sc ("Logic_Thms.iff_intro2", 1) *}
 
 (* Implies. *)
-theorem imp_intro: "\<not>(A \<longrightarrow> B) \<Longrightarrow> A \<and> \<not>B" by simp
-setup {* add_forward_prfstep @{thm imp_intro} *}
-setup {* add_fixed_sc ("Logic_Thms.imp_intro", 1) *}
+setup {* add_forward_prfstep @{thm Meson.not_impD} *}
+setup {* add_fixed_sc ("Meson.not_impD", 1) *}
 
-(* Quantifiers (proofsteps in ML). *)
+(* Quantifiers. *)
 theorem exists_intro: "\<not> (\<exists>x. P x \<and> Q x) \<Longrightarrow> P x \<Longrightarrow> \<not> (Q x)" by simp
-theorem exists_intro2: "\<not> (\<exists>x y. P x y \<and> Q x y) \<Longrightarrow> P x y \<Longrightarrow> \<not> (Q x y)" by simp
 theorem exists_resolve: "\<not> (\<exists>x. P x) \<Longrightarrow> P x \<Longrightarrow> False" by simp
-theorem forall_resolve0: "\<forall>x. P x \<Longrightarrow> \<not>(P x) \<Longrightarrow> False" by simp
-theorem forall_resolve0': "\<forall>x. \<not>(P x) \<Longrightarrow> P x \<Longrightarrow> False" by simp
-theorem forall_resolve: "\<forall>x. P x \<longrightarrow> Q x \<Longrightarrow> P x \<Longrightarrow> Q x" by simp
-theorem forall_resolve_opp: "\<forall>x. P x \<longrightarrow> \<not>(Q x) \<Longrightarrow> Q x \<Longrightarrow> \<not>(P x)" by blast
-theorem forall_resolve2: "\<forall>x y. P x y \<longrightarrow> Q x y \<Longrightarrow> P x y \<Longrightarrow> Q x y" by blast
-theorem forall_eq: "\<forall>x. P x = Q x \<Longrightarrow> P x \<equiv> Q x" by simp
-theorem forall_eq': "\<forall>x. P x = Q x \<Longrightarrow> Q x \<equiv> P x" by simp
-theorem forall_eq2: "\<forall>x y. P x y = Q x y \<Longrightarrow> P x y \<equiv> Q x y" by simp
-theorem forall_eq2': "\<forall>x y. P x y = Q x y \<Longrightarrow> Q x y \<equiv> P x y" by simp
+theorem forall_impl: "\<forall>x. P x \<longrightarrow> Q x \<Longrightarrow> P x \<Longrightarrow> Q x" by simp
+setup {* add_rewrite_rule @{thm HOL.not_all} *}
 
-(* Quantifiers: splitting (proofsteps in ML). *)
+(* Quantifiers: splitting. *)
+theorem forall_or: "(\<forall>x. ((A x \<or> B x) \<longrightarrow> C x)) \<Longrightarrow> ((\<forall>x. A x \<longrightarrow> C x) \<and> (\<forall>x. B x \<longrightarrow> C x))" by blast
+setup {* add_forward_prfstep @{thm forall_or} *}
 theorem exists_split: "(\<exists>x y. P x \<and> Q y) = ((\<exists>x. P x) \<and> (\<exists>y. Q y))" by simp
+setup {* add_rewrite_rule @{thm exists_split} *}
 theorem exists_split': "(\<exists>y x. P x \<and> Q y) = ((\<exists>x. P x) \<and> (\<exists>y. Q y))" by simp
-theorem forall_split1: "(\<forall>x y. P x \<and> Q y \<longrightarrow> R x y) = (\<forall>x. P x \<longrightarrow> (\<forall>y. Q y \<longrightarrow> R x y))" by smt
-theorem forall_split2: "(\<forall>x y. P x \<and> Q y \<longrightarrow> R x y) = (\<forall>y. Q y \<longrightarrow> (\<forall>x. P x \<longrightarrow> R x y))" by smt
-theorem forall_or: "(\<forall>x. ((A x \<or> B x) \<longrightarrow> C x)) = ((\<forall>x. A x \<longrightarrow> C x) \<and> (\<forall>x. B x \<longrightarrow> C x))" by blast
 
-(* (\<forall>x. ?t = x \<longrightarrow> ?P x) = ?P ?t *)
-setup {* add_eq_th_normalizer use_vardef_th *}
+(* (\<forall>x. x = ?t \<longrightarrow> ?P x) = ?P ?t *)
+setup {* add_eq_th_normalizer @{thm use_vardef} *}
 (* (\<forall>x. ?P \<longrightarrow> ?Q x) = (?P \<longrightarrow> (\<forall>x. ?Q x)) *)
 setup {* add_eq_th_normalizer @{thm HOL.all_simps(6)} *}
 
@@ -99,16 +80,10 @@ setup {* add_eq_th_normalizer @{thm HOL.all_simps(6)} *}
 setup {* add_gen_prfstep ("case_intro",
   [WithTerm @{term_pat "if ?cond then (?yes::?'a) else ?no"},
    CreateCase ([@{term_pat "?cond::bool"}], [])]) *}
-theorem if_true: "cond \<Longrightarrow> (if cond then yes else no) = yes" by (simp add: simp_eq_def)
-setup {* add_forward_prfstep_cond @{thm if_true} [with_term "if ?cond then ?yes else ?no"] *}
 theorem if_true': "(if a = a then yes else no) = yes" by simp
-setup {* add_simp_rule @{thm if_true'} *}
-theorem if_false: "\<not>cond \<Longrightarrow> (if cond then yes else no) = no" by simp
-setup {* add_forward_prfstep_cond @{thm if_false} [with_term "if ?cond then ?yes else ?no"] *}
 theorem if_false': "cond \<Longrightarrow> (if \<not>cond then yes else no) = no" by simp
-setup {* add_forward_prfstep_cond @{thm if_false'} [with_term "if \<not> ?cond then ?yes else ?no"] *}
-setup {* fold add_fixed_sc [("Logic_Thms.if_true", 1), ("Logic_Thms.if_true'", 1),
-                            ("Logic_Thms.if_false", 1), ("Logic_Thms.if_false'", 1)] *}
+setup {* fold add_rewrite_rule [@{thm HOL.if_P}, @{thm HOL.if_not_P}, @{thm if_false'}] *}
+setup {* fold add_fixed_sc [("HOL.if_P", 1), ("HOL.if_not_P", 1), ("Logic_Thms.if_false'", 1)] *}
 
 (* Quantifiers and other fundamental proofsteps. *)
 ML_file "logic_steps.ML"
